enact countability assumption (top operate on finite Types)

Structures/Blocks.v
@@ -1,5 +1,5 @@
 From mathcomp.ssreflect
-Require Import ssreflect ssrbool ssrnat eqtype fintype ssrfun seq path.
+Require Import ssreflect ssrbool ssrnat eqtype fintype ssrfun seq path choice.
 Require Import Eqdep.
 From fcsl
 Require Import pred prelude ordtype pcm finmap unionmap heap.
@@ -15,7 +15,27 @@ Unset Printing Implicit Defensive.
 Open Scope sign_scope.
 Section BlockType.
 
-Variable Hash: ordType.
+Variable Hash: countType.
+
+Definition pickle_ordering: rel [eqType of Hash] :=
+  fun h1 h2 => (pickle h1) < (pickle h2).
+
+Lemma pickle_irref: irreflexive pickle_ordering.
+Proof. by move => x; rewrite /pickle_ordering ltnn. Qed.
+Lemma pickle_trans: transitive pickle_ordering.
+Proof. by move => x y z; rewrite /pickle_ordering; apply ltn_trans. Qed.
+Lemma pickle_spec:  forall x y, [|| pickle_ordering x y, x == y | pickle_ordering y x].
+Proof. move => x y; rewrite /pickle_ordering.
+case H: (pickle x == pickle y).
+- move/pcan_inj: (@pickleK Hash); move/(_ _ _ (eqP H))/eqP=>->.
+  by rewrite orbT.
+by move/negbT: H; rewrite neq_ltn orbCA=>->; rewrite orbT.
+Qed.
+
+Definition hash_ordMixin := OrdMixin pickle_irref pickle_trans pickle_spec.
+Definition hash_ordType := OrdType _ hash_ordMixin.
+Canonical hash_ordType.
+
 
 Record VoteData := mkVD {
   block_hash: Hash;
@@ -25,14 +45,35 @@ Record VoteData := mkVD {
   parent_block_round: nat;
 }.
 
+
+Definition vote2nats (vd: VoteData) :=
+  (block_hash vd, executed_hash vd, block_round vd, parent_block_hash vd, parent_block_round vd).
+Definition nats2vote (nats: Hash * Hash * nat * Hash * nat) :=
+  let: (bh, eh, br, ph, pr) := nats in mkVD bh eh br ph pr.
+Lemma vote_nats_cancel: ssrfun.cancel vote2nats nats2vote.
+Proof. by move => []. Qed.
+
+Definition vote_data_eqMixin := CanEqMixin vote_nats_cancel.
+Canonical vote_data_eqType :=
+  Eval hnf in EqType _ vote_data_eqMixin.
+
+Definition vote_data_choiceMixin := CanChoiceMixin vote_nats_cancel.
+Canonical vote_data_choiceType :=
+  Eval hnf in ChoiceType _ vote_data_choiceMixin.
+
+Definition vote_data_countMixin := CanCountMixin vote_nats_cancel.
+Canonical  vote_data_countType :=
+  Eval hnf in CountType VoteData vote_data_countMixin.
+
 (* The VoteMsg assume there's a way to hash and sign VoteData*)
-Variables (PublicKey: Type) (Signature: eqType)
+(* The Pubkey, SignType are countTypes, reflecting they are serializable*)
+Variables (PublicKey: countType) (Signature: countType)
             (HashV: signType VoteData PublicKey Signature).
 
-Definition VD_eqMixin :=
-  Eval hnf in (InjEqMixin (@hash_inj _ HashV)).
-Canonical VD_eqType :=
-  Eval hnf in EqType _ VD_eqMixin.
+(* Definition VD_eqMixin := *)
+(*   Eval hnf in (InjEqMixin (@hash_inj _ HashV)). *)
+(* Canonical VD_eqType := *)
+(*   Eval hnf in EqType _ VD_eqMixin. *)
 
 Variable Address: hashType PublicKey.
 
@@ -41,10 +82,10 @@ Record VoteMsg (phA: phant Address) := mkVM {
   vote: (PublicKey * Signature);
 }.
 
-Definition PK_eqMixin :=
-  Eval hnf in InjEqMixin (@hash_inj _ Address).
-Canonical PK_eqType :=
-  Eval hnf in EqType _ PK_eqMixin.
+(* Definition PK_eqMixin := *)
+(*   Eval hnf in InjEqMixin (@hash_inj _ Address). *)
+(* Canonical PK_eqType := *)
+(*   Eval hnf in EqType _ PK_eqMixin. *)
 
 Definition vm2triple (v: VoteMsg (Phant Address)) :=
   let: mkVM vd pks := v in (vd, pks).
@@ -57,6 +98,13 @@ Proof. by move => []. Qed.
 
 Definition vm_eqMixin := CanEqMixin can_vm_triple.
 Canonical vm_eqType := EqType _ vm_eqMixin.
+
+Definition vm_choiceMixin := CanChoiceMixin can_vm_triple.
+Canonical vm_choiceType := ChoiceType _ vm_choiceMixin.
+
+Definition vm_countMixin := CanCountMixin can_vm_triple.
+Canonical vm_countType :=
+  Eval hnf in CountType _ vm_countMixin.
 
 Record QuorumCert (phA: phant Address) := mkQC {
   qc_vote_data: VoteData;
@@ -73,11 +121,19 @@ Proof. by move => []. Qed.
 Definition qc_eqMixin := CanEqMixin can_qc_votes.
 Canonical qc_eqType := EqType _ qc_eqMixin.
 
+Definition qc_choiceMixin := CanChoiceMixin can_qc_votes.
+Canonical qc_choiceType := ChoiceType _ qc_choiceMixin.
+
+Definition qc_countMixin := CanCountMixin can_qc_votes.
+Canonical qc_countType :=
+  Eval hnf in CountType _ qc_countMixin.
+
 (* We can finally define the block type *)
 
-(* The hashability implies the eqType*)
-Variable Command: Type.
-Variable NodeTime: Type.
+(* The hashability would imply the eqType, but we need serializability -> *)
+(* countType *)
+Variable Command: countType.
+Variable NodeTime: countType.
 
 Record BlockData := mkBD {
     (* Parent's hash pointer is in the QC *)
@@ -89,6 +145,23 @@ Record BlockData := mkBD {
     (* Parent's QC information *)
     proof : QuorumCert (Phant Address);
 }.
+
+Definition bd2qudruplet (bd: BlockData) :=
+  (txs bd, time bd, round bd, proof bd).
+Definition quadruplet2bd (q: seq Command * NodeTime * nat * QuorumCert(Phant Address)) :=
+  let: (tx, nt, r, pf) := q in mkBD tx nt r pf.
+Lemma cancel_bd_quadruplet: ssrfun.cancel bd2qudruplet quadruplet2bd.
+Proof. by move =>[]. Qed.
+
+Definition bd_eqMixin := CanEqMixin cancel_bd_quadruplet.
+Canonical bd_eqType := EqType _ bd_eqMixin.
+
+Definition bd_choiceMixin := CanChoiceMixin cancel_bd_quadruplet.
+Canonical bd_choiceType := ChoiceType _ bd_choiceMixin.
+
+Definition bd_countMixin := CanCountMixin cancel_bd_quadruplet.
+Canonical bd_countType :=
+  Eval hnf in CountType _ bd_countMixin.
 
 Record BlockType (hashB: BlockData -> Hash)(inj_hashB: injective hashB) (verifyB: Hash -> PublicKey -> Signature -> bool) := mkB {
   block_data: BlockData;
@@ -106,7 +179,7 @@ Definition Block_hashMixin :=
   Eval hnf in HashMixin hashB_inj.
 
 Canonical Block_hashType :=
-  Eval hnf in HashType BlockData Hash Block_hashMixin.
+  Eval hnf in HashType BlockData [ordType of Hash] Block_hashMixin.
 
 Variable verifB: Hash -> PublicKey -> Signature -> bool.
 
@@ -114,7 +187,7 @@ Definition Block_signMixin :=
   Eval hnf in SignMixin verifB.
 
 Canonical Block_signType :=
-  Eval hnf in SignType BlockData PublicKey Signature Hash Block_signMixin.
+  Eval hnf in SignType BlockData PublicKey Signature [ordType of Hash] Block_signMixin.
 
 Definition BD_eqMixin :=
   Eval hnf in (InjEqMixin (@hash_inj _ Block_hashType)).
@@ -130,6 +203,11 @@ Proof. by move => []. Qed.
 
 Definition bt_eqMixin := CanEqMixin can_bt_bdnsource.
 Canonical bt_eqType := EqType _ bt_eqMixin.
+Definition bt_choiceMixin := CanChoiceMixin can_bt_bdnsource.
+Canonical bt_choiceType := ChoiceType _ bt_choiceMixin.
+Definition bt_countMixin := CanCountMixin can_bt_bdnsource.
+Canonical bt_countType := CountType _ bt_countMixin.
+
 
 End BlockStructures.
 
